RelArchive.thy
@@ -1,0 +1,1287 @@
+theory RelArchive
+imports StmtRel
+begin 
+
+lemma method_call_stmt_rel_archived:
+  assumes WfConsistency: "wf_total_consistency ctxt_vpr StateCons StateCons_t"
+      and ConsistencyDownwardMono: "mono_prop_downward_ord StateCons"
+      and "Pr = program_total ctxt_vpr"
+          \<comment>\<open>We need to require state consistency, otherwise framing_exh cannot be established.\<close>
+      and ConsistencyEnabled: "consistent_state_rel_opt (state_rel_opt Tr)"
+      and MdeclSome:  "program.methods (program_total ctxt_vpr) m = Some mdecl"
+      and MethodSpecsFramed: "vpr_method_spec_correct_total ctxt_vpr StateCons mdecl"
+      and MethodSpecSubset:  "no_perm_assertion (method_decl.pre mdecl) \<and>                                    
+                              no_perm_assertion (method_decl.post mdecl) \<and> 
+                              no_unfolding_assertion (method_decl.pre mdecl) \<and>
+                              no_unfolding_assertion (method_decl.post mdecl)"
+      and OnlyArgsInPre: "\<And> x. x \<in> free_var_assertion (method_decl.pre mdecl) \<Longrightarrow> x < length es"
+      and "rtype_interp ctxt = []"
+      and DomainTyRep: "domain_type TyRep = absval_interp_total ctxt_vpr"
+      and TyInterpBplEq:   "type_interp ctxt = vbpl_absval_ty TyRep"
+      and StateRelConcrete: "\<And> \<omega> ns. R \<omega> ns \<Longrightarrow> state_rel_def_same Pr StateCons TyRep Tr AuxPred ctxt \<omega> ns"              
+      and ArgsAreVars: "list_all (\<lambda>x. \<exists>a. x = ViperLang.Var a) es" \<comment>\<open>simplifying assumption: only variables as arguments\<close>
+      and "xs = map the_var es"
+      and "set xs \<subseteq> dom (var_translation Tr)"
+      and XsBplEq: "map (the \<circ> var_translation Tr) xs = xs_bpl"
+      and "set ys \<subseteq> dom (var_translation Tr)"
+      and YsBplEq: "map (the \<circ> var_translation Tr) ys = ys_bpl"
+      and "set xs_bpl \<inter> set ys_bpl = {}" \<comment>\<open>simplifying assumption: targets and arguments do not clash\<close>
+      and "distinct xs" \<comment>\<open>simplifying assumption: arguments are distinct\<close>
+      and "distinct ys"
+             \<comment>\<open>TODO: One could probably track the following fact on declared types also via the variable relation
+                      where one ensures that the declared Viper and Boogie types match for variables related by
+                      the variable relation.\<close>
+      and LookupDeclRetsBpl: 
+                     "list_all2 (\<lambda>y_bpl t_vpr. \<exists>t_bpl. vpr_to_bpl_ty TyRep t_vpr = Some t_bpl \<and>
+                                           lookup_var_decl (var_context ctxt) y_bpl = Some (t_bpl, None))
+                                ys_bpl (method_decl.rets mdecl)"
+          \<comment>\<open> Since the rule only deals with variables in the arguments, well-definedness holds trivially
+             ExpWfRel: "exprs_wf_rel Rdef ctxt_vpr StateCons P ctxt es \<gamma> \<gamma>def"\<close>
+                   \<comment>\<open>simplifying assumption: unoptimized exhale and inhale\<close>
+                        \<comment>\<open>"var_tr' = [[0..<length es] [\<mapsto>] rev xs_bpl]" and \<close>
+      and "var_tr' = [[0..<length es] [\<mapsto>] xs_bpl]"
+      and ExhalePreRel:
+                      "\<And> fpred.                                                
+                        stmt_rel 
+                              (\<lambda>\<omega> ns.
+                                 state_rel_def_same Pr StateCons TyRep (Tr\<lparr> var_translation := var_tr' \<rparr>) (map_upd_set AuxPred (ran (var_translation Tr) - set xs_bpl) fpred) ctxt \<omega> ns \<and>
+                                 framing_exh ctxt_vpr StateCons (method_decl.pre mdecl) \<omega> \<omega>)
+                              (state_rel_def_same Pr StateCons TyRep (Tr\<lparr> var_translation := var_tr' \<rparr>) (map_upd_set AuxPred (ran (var_translation Tr) - set xs_bpl) fpred) ctxt) 
+                              ctxt_vpr StateCons \<Lambda>_vpr P ctxt 
+                              (Exhale (method_decl.pre mdecl)) \<gamma> (BigBlock name_pre cs_pre str_pre tr_pre, cont_pre)"
+      and "cs_pre = havocs_list_bpl ys_bpl @ cs_pre_suffix"
+      and "var_tr'' = Map.empty(upt 0 (length es+length ys) [\<mapsto>] (xs_bpl @ ys_bpl))"
+      and InhalePostRel: 
+          "\<And> fpred.  stmt_rel 
+                        (\<lambda> \<omega> ns. 
+                         state_rel_def_same Pr StateCons TyRep (Tr\<lparr> var_translation := var_tr'' \<rparr>) (map_upd_set AuxPred (ran (var_translation Tr) - (set xs_bpl \<union> set ys_bpl)) fpred) ctxt \<omega> ns \<and>
+                         assertion_framing_state ctxt_vpr StateCons (method_decl.post mdecl) \<omega> 
+                        )
+                        (state_rel_def_same Pr StateCons TyRep (Tr\<lparr> var_translation := var_tr'' \<rparr>) (map_upd_set AuxPred (ran (var_translation Tr) - (set xs_bpl \<union> set ys_bpl)) fpred) ctxt)
+                        ctxt_vpr StateCons \<Lambda>_vpr P ctxt 
+                        (Inhale (method_decl.post mdecl)) (BigBlock name_pre cs_pre_suffix str_pre tr_pre, cont_pre) \<gamma>'"
+      shows "stmt_rel R (state_rel_def_same Pr StateCons TyRep Tr AuxPred ctxt) ctxt_vpr StateCons \<Lambda>_vpr P ctxt (MethodCall ys m es) \<gamma> \<gamma>'"
+proof (rule stmt_rel_intro_2)
+  fix \<omega> ns res
+  assume "R \<omega> ns" 
+  \<comment>\<open>Prove various properties before showing the goal\<close>
+  hence StateRel: "state_rel_def_same Pr StateCons TyRep Tr AuxPred ctxt \<omega> ns"
+    using StateRelConcrete
+    by blast  
+
+  hence "StateCons_t (get_total_full \<omega>)"
+    using state_rel_consistent StateRel WfConsistency ConsistencyEnabled
+    unfolding wf_total_consistency_def
+    by blast
+    
+  have "es = map pure_exp.Var xs"
+  proof (rule nth_equalityI)
+    show "length es = length (map pure_exp.Var xs)"
+      using \<open>xs = _\<close>
+      by simp
+  next
+    fix i 
+    assume "i < length es"
+    show "es ! i = map pure_exp.Var xs ! i"
+    proof -
+      have "xs ! i = the_var (es ! i)"
+        using \<open>i < _\<close> \<open>xs = _\<close>
+        by simp
+      moreover from ArgsAreVars obtain x where
+          "es ! i = pure_exp.Var x"
+        using \<open>i < _\<close>                 
+        by (fastforce simp: list_all_length)
+
+      ultimately show ?thesis
+        using \<open>i < length es\<close> \<open>xs = _\<close> by auto
+    qed            
+  qed
+
+  have "set xs_bpl \<subseteq> ran (var_translation Tr)"
+  proof 
+    fix x_bpl
+    assume "x_bpl \<in> set xs_bpl"
+
+    from this obtain x_vpr where "x_vpr \<in> set xs" and "the ((var_translation Tr) x_vpr) = x_bpl"
+      using XsBplEq
+      by auto
+
+    moreover with \<open>set xs \<subseteq> dom (var_translation Tr)\<close> obtain x_bpl' where "var_translation Tr x_vpr = Some x_bpl'"
+      by fast
+
+    ultimately show "x_bpl \<in> ran (var_translation Tr)"
+      by (simp add: ranI)
+  qed
+
+  have "set ys_bpl \<subseteq> ran (var_translation Tr)"
+  proof 
+    fix x_bpl
+    assume "x_bpl \<in> set ys_bpl"
+
+    from this obtain x_vpr where "x_vpr \<in> set ys" and "the ((var_translation Tr) x_vpr) = x_bpl"
+      using YsBplEq
+      by auto
+
+    moreover with \<open>set ys \<subseteq> dom (var_translation Tr)\<close> obtain x_bpl' where "var_translation Tr x_vpr = Some x_bpl'"
+      by fast
+
+    ultimately show "x_bpl \<in> ran (var_translation Tr)"
+      by (simp add: ranI)
+  qed
+
+  have "distinct xs_bpl" and "distinct ys_bpl"
+  proof -
+    have "inj_on (var_translation Tr) (dom (var_translation Tr))"
+    using state_rel_store_rel[OF StateRelConcrete[OF \<open>R \<omega> ns\<close>]]
+    unfolding store_rel_def
+    by blast
+
+    thus "distinct ys_bpl" and "distinct xs_bpl"
+      using XsBplEq YsBplEq distinct_map_the_inj_on_subset \<open>distinct xs\<close> \<open>distinct ys\<close> \<open>set xs \<subseteq> _\<close> \<open>set ys \<subseteq> _\<close> 
+      by blast+
+  qed
+
+  \<comment>\<open>Show the goal\<close>
+
+  assume "red_stmt_total ctxt_vpr StateCons \<Lambda>_vpr (MethodCall ys m es) \<omega> res"
+
+  thus "rel_vpr_aux (state_rel_def_same Pr StateCons TyRep Tr AuxPred ctxt) P ctxt \<gamma> \<gamma>' ns res"
+  proof (cases)
+    case (RedMethodCall v_args mdecl' v_rets resPre resPost)
+     \<comment>\<open>All arguments evaluate normally\<close>
+
+    from MdeclSome RedMethodCall have "mdecl = mdecl'"
+      by force
+
+    have ListAllArgsEvalVpr: "list_all2 (\<lambda>e v. ctxt_vpr, StateCons, Some \<omega> \<turnstile> \<langle>e; \<omega>\<rangle> [\<Down>]\<^sub>t Val v) es v_args"
+      using red_pure_exps_total_list_all2 RedMethodCall
+      by blast
+
+    hence "length es = length v_args"
+      by (simp add: list_all2_lengthD)
+
+    have "length xs = length xs_bpl"
+      using XsBplEq
+      by auto
+
+    have "length xs_bpl = length v_args"
+      using RedMethodCall \<open>xs = _\<close> XsBplEq
+      by (metis ListAllArgsEvalVpr length_map list_all2_lengthD)    
+
+    have "length ys = length ys_bpl"
+      using YsBplEq by auto
+
+    hence "length ys_bpl = length v_rets"
+      using RedMethodCall
+      unfolding vals_well_typed_def
+      by (metis length_map list_all2_lengthD)
+
+    note LengthEqs = \<open>length es = length v_args\<close> \<open>length xs = length xs_bpl\<close> \<open>length xs_bpl = length v_args\<close>
+                     \<open>length ys = length ys_bpl\<close> \<open>length ys_bpl = length v_rets\<close>
+
+    have "list_all2 (\<lambda>x v. ctxt_vpr, StateCons, Some \<omega> \<turnstile> \<langle>ViperLang.Var x; \<omega>\<rangle> [\<Down>]\<^sub>t Val v) xs v_args"
+    proof (rule list_all2_all_nthI)
+      show "length xs = length v_args"
+        using LengthEqs
+        by simp
+    next
+      fix i
+      assume "i < length xs"
+     
+      hence *: "ctxt_vpr, StateCons, Some \<omega> \<turnstile> \<langle>es ! i; \<omega>\<rangle> [\<Down>]\<^sub>t Val (v_args ! i)"
+        using ListAllArgsEvalVpr LengthEqs
+        by (simp add: list_all2_conv_all_nth)
+
+      have "es ! i = pure_exp.Var (xs ! i)"
+        using \<open>i < _\<close> \<open>es = _\<close>
+        by auto
+  
+      thus "ctxt_vpr, StateCons, Some \<omega> \<turnstile> \<langle>pure_exp.Var (xs ! i);\<omega>\<rangle> [\<Down>]\<^sub>t Val (v_args ! i)"
+        using *
+        by simp
+    qed        
+
+    hence StoreValArgsVpr: "list_all2 (\<lambda>x v. get_store_total \<omega> x = Some v) xs v_args"
+      using TotalExpressions.RedVar_case
+      by (metis (mono_tags, lifting) list_all2_mono)
+
+    have StoreRelAuxArgs: 
+      "list_all2 (\<lambda> x_vpr x_bpl. store_var_rel_aux (type_interp ctxt) (var_context ctxt) \<omega> ns x_vpr x_bpl) xs xs_bpl"
+    proof (rule list_all2_all_nthI)
+      fix i
+      assume "i < length xs"
+
+      let ?x_vpr = "xs ! i"
+      let ?x_bpl = "xs_bpl ! i"
+
+
+      have "var_translation Tr (xs ! i) = Some (xs_bpl ! i)"
+        using XsBplEq \<open>set xs \<subseteq> dom _\<close> \<open>i < _\<close> nth_mem
+        by fastforce
+
+      thus "store_var_rel_aux (type_interp ctxt) (var_context ctxt) \<omega> ns ?x_vpr ?x_bpl"
+        using state_rel_store_rel[OF StateRelConcrete[OF \<open>R \<omega> ns\<close>]]
+        unfolding store_var_rel_aux_def store_rel_def
+        by blast 
+    next
+      show "length xs = length xs_bpl"
+        using XsBplEq by auto
+    qed
+
+    have ValRelArgs: "list_all2 
+          (\<lambda> v_vpr x_bpl. lookup_var (var_context ctxt) ns x_bpl = Some (val_rel_vpr_bpl v_vpr) \<and>
+                          (\<exists>ty_bpl. lookup_var_ty (var_context ctxt) x_bpl = Some ty_bpl \<and> 
+                          type_of_val (type_interp ctxt) (val_rel_vpr_bpl v_vpr) = ty_bpl)) 
+          v_args 
+          xs_bpl"
+    proof (rule list_all2_all_nthI)
+      show "length v_args = length xs_bpl"
+        by (simp add: \<open>length xs_bpl = length v_args\<close>)
+    next
+      fix i 
+      assume "i < length v_args"
+
+      with \<open>length xs_bpl = length v_args\<close> have
+        "store_var_rel_aux (type_interp ctxt) (var_context ctxt) \<omega> ns (xs ! i) (xs_bpl ! i)"
+        using StoreRelAuxArgs
+        by (metis list_all2_nthD2)
+
+      thus "lookup_var (var_context ctxt) ns (xs_bpl ! i) = Some (val_rel_vpr_bpl (v_args ! i)) \<and>
+         (\<exists>ty_bpl. lookup_var_ty (var_context ctxt) (xs_bpl ! i) = Some ty_bpl \<and> 
+         type_of_val (type_interp ctxt) (val_rel_vpr_bpl (v_args ! i)) = ty_bpl)"        
+        using StoreValArgsVpr \<open>i < _\<close>
+        unfolding store_var_rel_aux_def
+        by (simp add: list_all2_conv_all_nth)
+    qed
+
+      \<comment>\<open>Show state rel with new var translation, which is required to use the exhale relation on the
+         precondition\<close>
+
+    let ?\<omega>0 = "\<lparr>get_store_total = shift_and_add_list_alt Map.empty v_args, 
+                get_trace_total = [old_label \<mapsto> get_total_full \<omega>],
+                get_total_full = get_total_full \<omega>\<rparr>"
+
+    let ?fpred  = "(\<lambda>x. pred_eq (the (lookup_var (var_context ctxt) ns x)))"
+
+    note ExhalePreRelInst = ExhalePreRel
+    (*note InhalePostRelInst = InhalePostRel[OF \<open>set ls = _\<close> \<open>length ls = length ?ps\<close>]*)
+    let ?AuxPredPre = "(map_upd_set AuxPred (ran (var_translation Tr) - set xs_bpl) ?fpred)"
+    let ?RCall = "state_rel_def_same Pr StateCons TyRep (Tr\<lparr> var_translation := var_tr' \<rparr>) ?AuxPredPre ctxt"
+    have StateRelDuringCall: "?RCall ?\<omega>0 ns"
+    proof -
+      from var_translation_disjoint[OF StateRelConcrete[OF \<open>R \<omega> ns\<close>]] have 
+        *: "ran (var_translation Tr) \<inter> dom AuxPred = {}"
+        by blast
+
+      have AuxSub: "map_upd_set AuxPred (ran (var_translation Tr) - set xs_bpl) ?fpred \<subseteq>\<^sub>m
+            map_upd_set AuxPred (ran (var_translation Tr)) ?fpred"
+        unfolding map_upd_set_def
+        apply (rule map_add_le_dom_disjoint)
+        using *
+         apply (smt (verit) disjoint_iff_not_equal domIff)
+        by (smt (verit) Diff_iff domIff map_le_def)
+
+      have StoreRel: "store_rel (type_interp ctxt) (var_context ctxt) var_tr' ?\<omega>0 ns"
+      proof (rule store_relI)
+        \<comment>\<open>Could adjust state rel with an additional parameter that switches off injectivity on the variable translation.
+           Then, one could support multiple arguments being the same variable. Injectivity is useful only if there
+           are changes to the local Viper variables.\<close>
+        show "inj_on var_tr' (dom var_tr')"
+          unfolding \<open>var_tr' = _\<close>
+          using inj_on_upt_distinct \<open>distinct xs_bpl\<close> LengthEqs
+          by fastforce
+      next
+        fix x_vpr x_bpl
+        assume VarTrSome: "var_tr' x_vpr = Some x_bpl" 
+        with \<open>var_tr' = _\<close>
+        have "x_vpr \<in> set [0..<length es]"
+          by (metis Some_Some_ifD map_upds_apply_nontin)
+        hence "x_vpr < length es"
+          by simp
+        hence "x_vpr < length v_args"
+          using ListAllArgsEvalVpr
+          using list_all2_lengthD by force
+        with ValRelArgs
+        have *:"lookup_var (var_context ctxt) ns (xs_bpl ! x_vpr) = Some (val_rel_vpr_bpl ( v_args ! x_vpr))"
+          using list_all2_nthD 
+          by blast
+        
+        have "x_bpl = xs_bpl ! x_vpr"
+        proof -
+          from \<open>x_vpr \<in> _\<close> have *: "x_vpr = [0..<length es] ! x_vpr"
+            by simp
+          thus ?thesis
+            using map_upds_distinct_nth[OF distinct_upt *, where ?m=Map.empty and ?ys = "xs_bpl"]
+                  LengthEqs VarTrSome \<open>x_vpr < length v_args\<close> \<open>var_tr' = _\<close> 
+            by auto
+        qed          
+
+        hence "x_bpl \<in> set xs_bpl"
+          using \<open>x_vpr < length v_args\<close> \<open>length xs_bpl = length v_args\<close>
+          by force
+
+        from ValRelArgs obtain \<tau>_bpl where
+          XBplTy: "lookup_var_ty (var_context ctxt) x_bpl = Some \<tau>_bpl" 
+                  "type_of_val (type_interp ctxt) (val_rel_vpr_bpl (v_args ! x_vpr)) = \<tau>_bpl"
+          using  \<open>x_bpl = _\<close> \<open>x_vpr < length v_args\<close> list_all2_nthD by blast          
+
+        show "store_var_rel_aux (type_interp ctxt) (var_context ctxt) ?\<omega>0 ns x_vpr x_bpl"
+          unfolding store_var_rel_aux_def
+        proof ((rule exI)+, intro conjI)
+          show "get_store_total ?\<omega>0 x_vpr = Some (v_args ! x_vpr)"
+            using shift_and_add_list_alt_lookup_1 \<open>x_vpr < length v_args\<close>
+            by auto
+        next
+          from * \<open>x_bpl = _\<close> 
+          show "lookup_var (var_context ctxt) ns x_bpl = Some (val_rel_vpr_bpl (v_args ! x_vpr))"
+            by simp  
+        next
+          show "lookup_var_ty (var_context ctxt) x_bpl = Some \<tau>_bpl"
+            using XBplTy
+            by blast
+        next
+          show "type_of_val (type_interp ctxt) (val_rel_vpr_bpl (v_args ! x_vpr)) = \<tau>_bpl"
+            using XBplTy
+            by blast
+        qed
+      qed      
+
+      have "ran var_tr' = set xs_bpl"
+        using map_upds_upt_ran LengthEqs
+        unfolding \<open>var_tr' = _\<close>
+        by force
+  
+      have "state_rel Pr StateCons TyRep (Tr \<lparr> var_translation := Map.empty \<rparr>) ?AuxPredPre ctxt \<omega> \<omega> ns"
+        apply (rule state_rel_aux_pred_remove)
+         apply (rule state_rel_transfer_var_tr_to_aux_pred[OF StateRelConcrete[OF \<open>R \<omega> ns\<close>]])
+          apply simp
+          apply simp
+         apply simp
+        by (rule AuxSub)        
+
+      thus ?thesis
+      proof (rule state_rel_store_update[where ?f= var_tr'])
+        show "consistent_state_rel_opt (state_rel_opt (Tr\<lparr>var_translation := var_tr'\<rparr>)) \<Longrightarrow> StateCons ?\<omega>0"
+          apply (rule total_consistencyI[OF WfConsistency])
+           apply (insert \<open>StateCons_t (get_total_full \<omega>)\<close>)
+           apply (solves \<open>simp\<close>)
+          apply simp
+          by (metis option.distinct(1) option.inject)           
+      next
+        show "binder_state ns = Map.empty"
+          using state_rel_state_well_typed[OF StateRelConcrete[OF \<open>R \<omega> ns\<close>], simplified state_well_typed_def]
+          by simp
+      next
+        show "store_rel (type_interp ctxt) (var_context ctxt) var_tr' ?\<omega>0 ns"
+          using StoreRel
+          by blast
+      qed (insert  var_translation_disjoint[OF StateRelConcrete[OF \<open>R \<omega> ns\<close>]] \<open>set xs_bpl \<subseteq> _\<close> \<open>ran var_tr' = _\<close>,
+           auto simp add: map_upd_set_lookup_2)
+    qed
+
+    have StoreSameOnArgs: "\<And>x. x \<in> free_var_assertion (method_decl.pre mdecl) \<Longrightarrow>
+               shift_and_add_list_alt Map.empty (v_args @ v_rets) x = 
+               shift_and_add_list_alt Map.empty v_args x" (is "\<And>x. _ \<Longrightarrow> ?store_args_rets x = ?store_args x")
+    proof -
+      fix x 
+      assume "x \<in> free_var_assertion (method_decl.pre mdecl)"
+      hence *: "x < length v_args"
+        using OnlyArgsInPre LengthEqs
+        by auto
+      hence **: "x < length (v_args @ v_rets)"
+        by simp
+
+      thus "?store_args_rets x = ?store_args x"
+      proof -
+        have "shift_and_add_list_alt Map.empty (v_args @ v_rets) x = Some ((v_args @ v_rets) ! x)"
+          using shift_and_add_list_alt_lookup_1[OF **]
+          by blast
+        also have "... = Some (v_args ! x)"
+          using \<open>x < length v_args\<close>
+          by (simp add: nth_append)
+        finally show "shift_and_add_list_alt Map.empty (v_args @ v_rets) x = shift_and_add_list_alt Map.empty v_args x"
+          using shift_and_add_list_alt_lookup_1[OF \<open>x < length v_args\<close>]
+          by simp
+      qed
+    qed
+    
+    have AssertionFramingInit: "framing_exh ctxt_vpr StateCons (method_decl.pre mdecl) ?\<omega>0 ?\<omega>0"
+    proof -
+      let ?\<omega>0_rets_empty = "\<lparr> get_store_total = shift_and_add_list_alt Map.empty (v_args@v_rets), 
+                    get_trace_total = [old_label \<mapsto> get_total_full \<omega>], 
+                    get_total_full = (get_total_full \<omega>)\<lparr> get_mh_total := zero_mask, get_mp_total := zero_mask \<rparr> \<rparr>"
+      let ?\<omega>0_empty = "?\<omega>0\<lparr> get_total_full := (get_total_full \<omega>)\<lparr> get_mh_total := zero_mask, get_mp_total := zero_mask \<rparr> \<rparr>"
+
+      have "assertion_framing_state ctxt_vpr StateCons (method_decl.pre mdecl) ?\<omega>0_rets_empty"
+        unfolding assertion_framing_state_def
+      proof (rule allI, rule impI)+
+        fix res
+        assume "red_inhale ctxt_vpr StateCons (method_decl.pre mdecl) ?\<omega>0_rets_empty res"           
+        moreover have "vpr_store_well_typed (absval_interp_total ctxt_vpr) (nth_option (method_decl.args mdecl @ rets mdecl)) (shift_and_add_list_alt Map.empty (v_args@v_rets))"
+          apply (rule vpr_store_well_typed_append)
+          using RedMethodCall \<open>mdecl = mdecl'\<close>
+          by (auto dest: vals_well_typed_same_lengthD)
+        moreover have "total_heap_well_typed (program_total ctxt_vpr) (absval_interp_total ctxt_vpr) (get_hh_total_full ?\<omega>0_rets_empty)"
+          using state_rel_heap_var_rel[OF StateRel] \<open>Pr = _\<close> \<open>domain_type TyRep = _\<close>
+          unfolding heap_var_rel_def
+          by simp
+        moreover have "is_empty_total_full ?\<omega>0_rets_empty"
+          by (simp add: is_empty_total_full_def is_empty_total_def)
+        ultimately show "res \<noteq> RFailure"
+          using MethodSpecsFramed
+          unfolding vpr_method_spec_correct_total_def vpr_method_correct_total_aux_def
+          by (metis full_total_state.select_convs(1))          
+      qed
+
+      hence AssertionFraming_\<omega>0'_only_args: "assertion_framing_state ctxt_vpr StateCons (method_decl.pre mdecl) ?\<omega>0_empty"
+     \<comment>\<open>using that return variables do not appear in precondition\<close>
+        apply (rule assertion_framing_store_same_on_free_var)
+        apply (insert StoreSameOnArgs, insert MethodSpecSubset)
+        by auto
+
+      show ?thesis        
+      proof (rule framing_exhI[OF _ _ AssertionFraming_\<omega>0'_only_args])
+        show "StateCons ?\<omega>0"
+          using StateRelDuringCall state_rel_consistent ConsistencyEnabled
+          by fastforce
+      next
+        show "valid_heap_mask (get_mh_total_full ?\<omega>0)"
+          using StateRelDuringCall state_rel_wf_mask_simple
+          by fast
+      next        
+        show "?\<omega>0_empty \<oplus> ?\<omega>0 = Some ?\<omega>0"
+          by (rule plus_full_total_state_zero_mask) simp_all          
+      next
+        show "?\<omega>0 \<succeq> ?\<omega>0"
+          by (simp add: succ_refl)
+      qed
+    qed
+
+    note RCallPre = conjI[OF \<open>?RCall ?\<omega>0 ns\<close> AssertionFramingInit]
+
+    show ?thesis 
+    proof (cases "resPre")
+      case RMagic
+      then show ?thesis \<comment>\<open>trivial case\<close>
+        using RedMethodCall
+        by (auto intro: rel_vpr_aux_intro)
+    next
+      case RFailure
+      with RedMethodCall \<open>mdecl = _\<close> 
+      obtain c where 
+          "red_ast_bpl P ctxt (\<gamma>, Normal ns) c" and
+          "snd c = Failure"
+        using stmt_rel_failure_elim[OF ExhalePreRelInst RCallPre]
+        by blast
+      moreover have "res = RFailure"
+        using RFailure RedMethodCall
+        by argo
+      ultimately show ?thesis         
+        using red_ast_bpl_transitive
+        by (blast intro: rel_vpr_aux_intro)                  
+    next
+      case (RNormal \<omega>pre)
+      let ?\<gamma>pre = "(BigBlock name_pre cs_pre str_pre tr_pre, cont_pre)"
+      from RNormal RedMethodCall \<open>mdecl = _\<close>
+      obtain nspre where
+        RedBplPre: "red_ast_bpl P ctxt (\<gamma>, Normal ns) (?\<gamma>pre, Normal nspre)" and
+        "?RCall \<omega>pre nspre"
+        using stmt_rel_normal_elim[OF ExhalePreRelInst RCallPre]
+        by blast
+
+      let ?\<omega>havoc = "\<lparr> get_store_total = (shift_and_add_list_alt Map.empty (v_args@v_rets)), 
+                       get_trace_total = [old_label \<mapsto> get_total_full \<omega>], 
+                       get_total_full = get_total_full \<omega>pre \<rparr>"
+ 
+      note InhalePostRelInst = InhalePostRel
+
+      let ?AuxPredPost = "(map_upd_set AuxPred (ran (var_translation Tr) - (set xs_bpl \<union> set ys_bpl)) ?fpred)"
+      let ?RCallPost = "state_rel_def_same Pr StateCons TyRep (Tr\<lparr> var_translation := var_tr'' \<rparr>) ?AuxPredPost ctxt"
+
+      let ?v_rets_bpl = "map (val_rel_vpr_bpl) v_rets"
+
+      let ?nshavoc = "update_var_list (var_context ctxt) nspre ys_bpl ?v_rets_bpl"
+
+      have *: "length ys_bpl = length (map val_rel_vpr_bpl v_rets)"
+      proof -
+          have "length ys = length ys_bpl"
+            using YsBplEq by auto
+          moreover have "length ys = length v_rets"
+            using RedMethodCall
+            unfolding vals_well_typed_def
+            by (metis length_map list_all2_lengthD)
+          ultimately show ?thesis
+            by simp
+        qed
+
+      have YsBplCorrectTypes: "list_all2 (\<lambda>x v. lookup_var_decl (var_context ctxt) x = Some (type_of_val (type_interp ctxt) v, None)) 
+                                     ys_bpl 
+                                     (map val_rel_vpr_bpl v_rets)"
+        proof (rule list_all2_all_nthI[OF *])        
+          fix n
+          assume "n < length ys_bpl"
+          
+          from this obtain t_bpl where 
+            "vpr_to_bpl_ty TyRep ((rets mdecl) ! n) = Some t_bpl"
+            "lookup_var_decl (var_context ctxt) (ys_bpl ! n) = Some (t_bpl, None)"
+            using LookupDeclRetsBpl
+            by (blast dest: list_all2_nthD)
+
+          moreover have "get_type (absval_interp_total ctxt_vpr) (v_rets ! n) = (rets mdecl) ! n"
+            using * \<open>n < _\<close> \<open>vals_well_typed (absval_interp_total ctxt_vpr) v_rets (rets mdecl')\<close>
+            unfolding vals_well_typed_def  \<open>mdecl = mdecl'\<close>
+            by (metis length_map nth_map)           
+
+          ultimately 
+         show "lookup_var_decl (var_context ctxt) (ys_bpl ! n) = 
+                 Some (type_of_val (type_interp ctxt) (map val_rel_vpr_bpl v_rets ! n), None)"
+           apply simp
+           using DomainTyRep vpr_to_bpl_val_type TyInterpBplEq 
+           by (metis "*" \<open>n < length ys_bpl\<close> list_update_id list_update_same_conv map_update)
+       qed
+
+      have
+        RedBplHavoc: "red_ast_bpl P ctxt (?\<gamma>pre, Normal nspre) ((BigBlock name_pre cs_pre_suffix str_pre tr_pre, cont_pre), Normal ?nshavoc)"
+        unfolding \<open>cs_pre = _\<close>
+      proof (rule red_ast_bpl_havoc_list, simp add: \<open>rtype_interp ctxt = _\<close>)   
+        show "list_all2 (\<lambda>x v. lookup_var_decl (var_context ctxt) x = Some (type_of_val (type_interp ctxt) v, None)) ys_bpl (map val_rel_vpr_bpl v_rets)"
+          using YsBplCorrectTypes
+          by simp
+      qed
+
+     have "ran var_tr'' = set xs_bpl \<union> set ys_bpl"
+       using LengthEqs map_upds_ran_distinct
+       unfolding \<open>var_tr'' = _\<close>
+       by (simp add: map_upds_upt_ran)
+
+     from \<open>?RCall \<omega>pre nspre\<close> have
+       "state_rel_def_same Pr StateCons TyRep (Tr\<lparr>var_translation := var_tr'\<rparr>)
+          (map_upd_set AuxPred (ran (var_translation Tr) - (set xs_bpl \<union> set ys_bpl)) (\<lambda>x. pred_eq (the (lookup_var (var_context ctxt) ns x)))) ctxt \<omega>pre nspre"
+       apply (rule state_rel_aux_pred_remove)
+       apply (rule map_upd_set_subset)
+        apply blast
+       using var_translation_disjoint[OF StateRelConcrete[OF \<open>R \<omega> ns\<close>]]
+       by blast
+
+     hence
+      "?RCallPost ?\<omega>havoc ?nshavoc"
+     proof (rule state_rel_store_update[where ?f=var_tr''])
+       fix x
+       assume "x \<notin> ran var_tr''"
+       hence "x \<notin> set ys_bpl"
+         using \<open>ran var_tr'' = _\<close>
+         by blast
+
+       thus "lookup_var (var_context ctxt) nspre x = 
+             lookup_var (var_context ctxt) (update_var_list (var_context ctxt) nspre ys_bpl (map val_rel_vpr_bpl v_rets)) x"
+         using lookup_update_var_list_other LengthEqs
+         by (metis length_map)
+     next
+       show "store_rel (type_interp ctxt) (var_context ctxt) var_tr'' ?\<omega>havoc ?nshavoc"
+       proof (rule store_relI)
+         show "inj_on var_tr'' (dom var_tr'')"
+         proof -
+           have *: "distinct (xs_bpl @ ys_bpl)"
+             using \<open>distinct xs_bpl\<close> \<open>distinct ys_bpl\<close> \<open>set xs_bpl \<inter> set ys_bpl = {}\<close>
+                   distinct_append
+             by blast
+
+           thus ?thesis
+             using LengthEqs inj_on_upt_distinct[OF *]
+             unfolding \<open>var_tr'' = _\<close>
+             by simp
+         qed        
+       next
+         fix var_vpr var_bpl
+         assume VarTrSome: "var_tr'' var_vpr = Some var_bpl"
+
+         with \<open>var_tr'' = _\<close>
+         have "var_vpr \<in> dom [[0..<length es + length ys] [\<mapsto>] xs_bpl @ ys_bpl]"
+           by (fastforce intro: domI)
+         hence "var_vpr < length es + length ys"
+           using map_upds_dom LengthEqs
+           by simp
+
+         hence "var_vpr = [0..<length es + length ys] ! var_vpr"
+           by simp
+
+         from VarTrSome \<open>var_tr'' = _\<close> 
+         have VarBplEqNth: "var_bpl = (xs_bpl @ ys_bpl) ! var_vpr"
+           using LengthEqs \<open>var_vpr < length es + length ys\<close>
+                 map_upds_distinct_nth[OF distinct_upt \<open>var_vpr = _\<close>, where ?m=Map.empty and ?ys="xs_bpl @ ys_bpl"]
+           by force
+
+         have HavocStoreVprLookupAux: "get_store_total ?\<omega>havoc var_vpr = Some ((v_args @ v_rets) ! var_vpr)"
+             apply (simp add: shift_and_add_list_alt_lookup)
+             using \<open>var_vpr < _\<close> LengthEqs
+             by linarith
+
+         show "store_var_rel_aux (type_interp ctxt) (var_context ctxt) ?\<omega>havoc ?nshavoc var_vpr var_bpl"
+         proof (cases "var_vpr < length es")
+           case True
+             \<comment>\<open>Prove facts properties \<^term>\<open>var_bpl\<close>\<close>
+             hence "var_bpl = xs_bpl ! var_vpr"
+               using VarBplEqNth LengthEqs
+               by (simp add: nth_append) 
+             hence "var_bpl \<in> set xs_bpl"
+               using LengthEqs True
+               by simp
+             hence LookupVarBplAux: "lookup_var (var_context ctxt) ?nshavoc var_bpl = lookup_var (var_context ctxt) nspre var_bpl"
+               using \<open>set xs_bpl \<inter> set ys_bpl = {}\<close> lookup_update_var_list_other LengthEqs
+               by (metis Int_iff empty_iff length_map)
+
+             have "var_tr' var_vpr = Some (xs_bpl ! var_vpr)"
+             proof -
+               have *: "var_vpr = [0..<length es] ! var_vpr"
+                 using True
+                 by simp
+               show ?thesis
+               unfolding \<open>var_tr' = _\<close>
+               using map_upds_distinct_nth[OF distinct_upt *, where ?m=Map.empty and ?ys="xs_bpl"]
+                     LengthEqs True
+               by fastforce
+             qed
+
+             with state_rel_store_rel[OF \<open>?RCall \<omega>pre nspre\<close>] 
+             obtain ty_bpl where
+                  VarBplValRel: "lookup_var (var_context ctxt) nspre var_bpl = Some (val_rel_vpr_bpl (the (get_store_total \<omega>pre var_vpr)))" and
+                  LookupTyVarBpl: "lookup_var_ty (var_context ctxt) var_bpl = Some ty_bpl" and
+                  TypeOfValRel:  "type_of_val (type_interp ctxt) (val_rel_vpr_bpl (the (get_store_total \<omega>pre var_vpr))) = ty_bpl"
+               using \<open>var_bpl = xs_bpl ! var_vpr\<close>
+               unfolding store_rel_def
+               by fastforce
+
+             from RedMethodCall have \<comment>\<open>exhale does not change the store\<close>
+                 StorePreVprEq: "get_store_total \<omega>pre = shift_and_add_list_alt Map.empty v_args"
+               using \<open>resPre = _\<close> exhale_only_changes_total_state
+               by force
+                 
+             hence StorePreVprEqLookup: "get_store_total \<omega>pre var_vpr = Some (v_args ! var_vpr)"
+               using True LengthEqs
+               by (simp add: shift_and_add_list_alt_lookup_1)
+
+             show "store_var_rel_aux (type_interp ctxt) (var_context ctxt) ?\<omega>havoc ?nshavoc var_vpr var_bpl"
+               unfolding store_var_rel_aux_def
+             proof ( (rule exI)+, intro conjI, rule HavocStoreVprLookupAux)
+               from StorePreVprEqLookup
+               show "lookup_var (var_context ctxt) ?nshavoc var_bpl =
+                     Some (val_rel_vpr_bpl ((v_args @ v_rets) ! var_vpr))" 
+               using VarBplValRel LookupVarBplAux True LengthEqs
+               by (simp add: nth_append)
+             next
+               show "lookup_var_ty (var_context ctxt) var_bpl = Some ty_bpl"
+                 by (rule LookupTyVarBpl)
+             next
+               show "type_of_val (type_interp ctxt) (val_rel_vpr_bpl ((v_args @ v_rets) ! var_vpr)) = ty_bpl"
+                 using TypeOfValRel StorePreVprEqLookup LengthEqs
+                 by (metis True nth_append option.sel)
+             qed
+         next
+           case False
+           hence VarVprLength: "var_vpr \<ge> length es \<and> var_vpr < length es + length ys"
+             using \<open>var_vpr < _\<close>
+             by simp
+
+           hence "(xs_bpl @ ys_bpl) ! var_vpr = ys_bpl ! (var_vpr - length xs_bpl)"
+             using LengthEqs
+             by (simp add: nth_append)
+
+           hence VarBplYsBplNth: "var_bpl = ys_bpl ! (var_vpr - length xs_bpl)" (is "_ = _ ! ?id_bpl")
+             using \<open>var_bpl  = _\<close>
+             by blast
+
+           hence "var_bpl \<in> set ys_bpl"
+             using VarVprLength LengthEqs
+             by fastforce
+
+           from VarBplYsBplNth obtain t_bpl where 
+              LookupDeclVarBpl: 
+                  "vpr_to_bpl_ty TyRep ((rets mdecl) ! ?id_bpl) = Some t_bpl \<and> 
+                   lookup_var_decl (var_context ctxt) var_bpl = Some (t_bpl, None)"
+             using list_all2_nthD[OF LookupDeclRetsBpl] VarVprLength LengthEqs
+             by fastforce
+
+           have *: "((v_args @ v_rets) ! var_vpr) = v_rets ! (var_vpr - length xs_bpl)" (is "_ = ?val_vpr")
+             using LengthEqs VarVprLength
+             by (simp add: nth_append)
+
+           have "?id_bpl < length ys_bpl"
+             using VarVprLength LengthEqs
+             by linarith
+
+           show ?thesis
+             unfolding store_var_rel_aux_def
+           proof ((rule exI)+, intro conjI, rule HavocStoreVprLookupAux)
+             show "lookup_var (var_context ctxt) ?nshavoc var_bpl = Some (val_rel_vpr_bpl ((v_args @ v_rets) ! var_vpr))" (is "?lhs = ?rhs")
+             proof -
+
+               have "?lhs = [ ys_bpl [\<mapsto>] (map val_rel_vpr_bpl v_rets) ] var_bpl"
+                 apply (rule lookup_update_var_list_same[ OF \<open>var_bpl \<in> _\<close> ])
+                 using LengthEqs
+                 by simp
+               also have "... = Some ((map val_rel_vpr_bpl v_rets) ! (var_vpr - length xs_bpl))"
+                 apply (rule map_upds_distinct_nth)
+                 using \<open>distinct ys_bpl\<close>
+                    apply simp
+                   apply (simp add: VarBplYsBplNth)
+                 using LengthEqs VarVprLength
+                  apply fastforce
+                 using LengthEqs
+                 by simp
+
+               finally show ?thesis                 
+                 using * VarVprLength LengthEqs nth_map
+                 by fastforce                 
+             qed
+           next
+             show "lookup_var_ty (var_context ctxt) var_bpl = Some t_bpl"
+               using LookupDeclVarBpl
+               by (simp add: lookup_var_decl_ty_Some)
+           next         
+             from YsBplCorrectTypes
+             have "lookup_var_decl (var_context ctxt) (ys_bpl ! ?id_bpl) = Some (type_of_val (type_interp ctxt) (val_rel_vpr_bpl ?val_vpr), None)"
+               using \<open>?id_bpl < _\<close>
+               by (simp add: list_all2_conv_all_nth rev_map)
+
+             hence "type_of_val (type_interp ctxt) (val_rel_vpr_bpl ?val_vpr) = t_bpl" 
+               using LookupDeclVarBpl VarBplYsBplNth
+               by simp
+
+             thus "type_of_val (type_interp ctxt) (val_rel_vpr_bpl ((v_args @ v_rets) ! var_vpr)) = t_bpl"
+               using *
+               by simp
+           qed
+         qed
+       qed
+     next
+       note aux_disj_thms = var_translation_disjoint[OF StateRelConcrete[OF \<open>R \<omega> ns\<close>]] 
+              \<open>set xs_bpl \<subseteq> _\<close> \<open>set ys_bpl \<subseteq> _\<close> \<open>ran var_tr'' = _\<close>
+       show "ran var_tr'' \<inter>
+            ({heap_var (Tr\<lparr>var_translation := var_tr'\<rparr>), heap_var_def (Tr\<lparr>var_translation := var_tr'\<rparr>)} \<union>
+             {mask_var (Tr\<lparr>var_translation := var_tr'\<rparr>), mask_var_def (Tr\<lparr>var_translation := var_tr'\<rparr>)} \<union>
+             ran (field_translation (Tr\<lparr>var_translation := var_tr'\<rparr>)) \<union>
+             range (const_repr (Tr\<lparr>var_translation := var_tr'\<rparr>)) \<union>
+             dom (map_upd_set AuxPred (ran (var_translation Tr) - (set xs_bpl \<union> set ys_bpl))
+                   (\<lambda>x. pred_eq (the (lookup_var (var_context ctxt) ns x))))) = {}"
+         apply simp
+         apply (intro conjI)
+
+         using aux_disj_thms
+             apply blast
+         using aux_disj_thms
+            apply blast
+         using aux_disj_thms
+           apply blast
+         using aux_disj_thms
+          apply blast
+         using aux_disj_thms
+         by (auto simp add: map_upd_set_dom)
+     next 
+       have "StateCons_t (get_total_full \<omega>pre)"
+       proof -
+         have "consistent_state_rel_opt (state_rel_opt (Tr\<lparr>var_translation := var_tr'\<rparr>))"
+           by (simp add: ConsistencyEnabled)
+         with state_rel_consistent[OF \<open>?RCall \<omega>pre nspre\<close>]  WfConsistency 
+         show ?thesis
+           unfolding wf_total_consistency_def
+           by blast
+       qed                  
+
+       show "StateCons
+              \<lparr> get_store_total = shift_and_add_list_alt Map.empty (v_args @ v_rets), 
+                get_trace_total = [old_label \<mapsto> get_total_full \<omega>],
+                get_total_full = get_total_full \<omega>pre \<rparr>"
+         apply (rule total_consistencyI[OF WfConsistency])
+          apply (simp add: \<open>StateCons_t (get_total_full \<omega>pre)\<close>)          
+         apply simp
+         by (fastforce  split: if_split_asm intro: \<open>StateCons_t (get_total_full \<omega>)\<close> )         
+     next
+       fix x
+       assume "map_of (snd (var_context ctxt)) x \<noteq> None"
+       thus "global_state ?nshavoc x = global_state nspre x"
+         using global_state_update_var_list_local 
+         by blast
+     next
+       show "old_global_state ?nshavoc = old_global_state nspre"
+         by (simp add: update_var_list_old_global_state_same)
+     next
+       show "binder_state ?nshavoc = Map.empty"
+         using state_rel_state_well_typed[OF \<open>?RCall \<omega>pre nspre\<close>, simplified state_well_typed_def]
+         by (simp add: update_var_list_binder_state_same)
+     qed simp_all
+
+      from RedMethodCall RNormal have 
+         RedInh: "red_stmt_total ctxt_vpr StateCons \<Lambda>_vpr (Inhale (method_decl.post mdecl')) ?\<omega>havoc resPost" and
+         "res = map_stmt_result_total (reset_state_after_call ys v_rets \<omega>) resPost"
+        by blast+
+
+      have PostFramed: "assertion_framing_state ctxt_vpr StateCons (method_decl.post mdecl) ?\<omega>havoc"       
+      proof -
+        \<comment>\<open>We know that the postcondition is framed w.r.t. the precondition. More precisely, the assumption
+           tells us that \<^emph>\<open>if\<close> the precondition is normally inhaled from an empty state \<^term>\<open>\<omega>_empty\<close> to reach \<^term>\<open>\<omega>inh\<close>, then the postcondition
+           is framed in any well-typed state whose store is the same as \<^term>\<open>get_store_total \<omega>_empty\<close> and whose old state is given 
+           by \<^term>\<open>\<omega>inh\<close>.
+
+           We first show that we can inhale the precondition from an empty state to reach \<^term>\<open>RNormal (?\<omega>0 \<ominus> \<omega>pre)\<close>
+           using the fact that the precondition was successfully exhaled from \<^term>\<open>?\<omega>0\<close> to reach \<^term>\<open>\<omega>pre\<close>.
+           From this, we will then learn that the postcondition is framed in
+           \<^term>\<open>?\<omega>havoc \<lparr> get_trace_total := [old_label \<mapsto> get_total_full (?\<omega>0 \<ominus> \<omega>pre)] \<rparr> \<close>.
+           From this we conclude the proof with a monotonicity argument (using that 
+           \<^prop>\<open>get_total_full ?\<omega>0 \<succeq> get_total_full (?\<omega>0 \<ominus> \<omega>pre)\<close>)\<close>        
+
+        let ?\<omega>0_rets =  "?\<omega>0\<lparr> get_store_total := shift_and_add_list_alt Map.empty (v_args@v_rets) \<rparr>"
+        let ?\<omega>0_rets_empty = "?\<omega>0\<lparr>   get_store_total := shift_and_add_list_alt Map.empty (v_args@v_rets),
+                                      get_total_full := (get_total_full \<omega>)\<lparr> get_mh_total := zero_mask, get_mp_total := zero_mask \<rparr> \<rparr>" 
+
+        let ?\<omega>pre_rets = "\<omega>pre \<lparr> get_store_total := shift_and_add_list_alt Map.empty (v_args@v_rets) \<rparr>"
+        from \<open>red_stmt_total ctxt_vpr StateCons \<Lambda>_vpr (Exhale (method_decl.pre mdecl')) ?\<omega>0 resPre\<close> 
+        obtain \<omega>pre_exh_aux where
+          RedExh: "red_exhale ctxt_vpr StateCons ?\<omega>0 (method_decl.pre mdecl') ?\<omega>0 (RNormal \<omega>pre_exh_aux)"
+          using \<open>resPre = _\<close>
+          by (cases) auto 
+
+        hence "?\<omega>0 \<succeq> \<omega>pre_exh_aux"
+          using exhale_normal_result_smaller
+          by blast
+
+        let ?\<omega>pre_exh_aux_rets = "\<omega>pre_exh_aux\<lparr> get_store_total := shift_and_add_list_alt Map.empty (v_args@v_rets) \<rparr>"
+
+        have "?\<omega>0_rets \<succeq> ?\<omega>pre_exh_aux_rets"
+        proof -
+          have TraceEq: "get_trace_total ?\<omega>0_rets = get_trace_total ?\<omega>pre_exh_aux_rets"
+            using exhale_only_changes_total_state_aux[OF RedExh]
+            by auto
+
+          have *: "?\<omega>0_rets \<ge> ?\<omega>pre_exh_aux_rets"
+            apply (rule less_eq_full_total_stateI)
+               apply simp
+            using TraceEq
+              apply simp
+              apply simp
+            using full_total_state_succ_implies_gte[OF \<open>?\<omega>0 \<succeq> \<omega>pre_exh_aux\<close>] less_eq_full_total_stateD
+            apply fastforce
+            by simp
+          show ?thesis 
+            using full_total_state_gte_implies_succ[OF *] TraceEq
+            by argo
+        qed
+
+        have StoreWellTy: "vpr_store_well_typed (absval_interp_total ctxt_vpr) (nth_option (method_decl.args mdecl @ rets mdecl)) (get_store_total ?\<omega>0_rets_empty)"
+          apply simp
+          apply (rule vpr_store_well_typed_append)
+          using RedMethodCall \<open>mdecl = mdecl'\<close>
+          by (auto dest: vals_well_typed_same_lengthD)
+        moreover have HeapWellTy: "total_heap_well_typed (program_total ctxt_vpr) (absval_interp_total ctxt_vpr) (get_hh_total_full ?\<omega>0_rets_empty)"
+          using state_rel_heap_var_rel[OF StateRel] \<open>Pr = _\<close> \<open>domain_type TyRep = _\<close>
+          unfolding heap_var_rel_def
+          by simp
+        moreover have EmptyState: "is_empty_total_full ?\<omega>0_rets_empty"
+          unfolding is_empty_total_full_def is_empty_total_def
+          by auto
+        moreover have "red_inhale ctxt_vpr StateCons (method_decl.pre mdecl) ?\<omega>0_rets_empty (RNormal (?\<omega>0_rets \<ominus> ?\<omega>pre_exh_aux_rets))"
+        proof -
+          have RedExhRets: "red_exhale ctxt_vpr StateCons ?\<omega>0_rets (method_decl.pre mdecl') ?\<omega>0_rets (RNormal ?\<omega>pre_exh_aux_rets)"
+            apply (rule exhale_same_on_free_var[OF RedExh]) \<comment>\<open>using that the return variables do not appear in the precondition\<close>
+            using StoreSameOnArgs \<open>mdecl = _\<close> MethodSpecSubset
+            by auto
+
+          moreover have SumDefined: "?\<omega>0_rets_empty \<oplus> (?\<omega>0_rets \<ominus> ?\<omega>pre_exh_aux_rets) = Some (?\<omega>0_rets \<ominus> ?\<omega>pre_exh_aux_rets)"
+          proof -
+            have "get_h_total_full (?\<omega>0_rets \<ominus> ?\<omega>pre_exh_aux_rets) = get_h_total_full ?\<omega>0_rets"
+            using minus_full_total_state_only_mask_different
+            by blast
+            hence *: "get_h_total_full (?\<omega>0_rets \<ominus> ?\<omega>pre_exh_aux_rets) = get_h_total_full ?\<omega>0_rets_empty"
+              by simp
+
+            show ?thesis
+              apply (rule plus_full_total_state_zero_mask)
+               apply (simp add: minus_full_total_state_only_mask_different)
+              using *
+               apply simp
+              by simp
+          qed
+          moreover have PreFramed: "assertion_framing_state ctxt_vpr StateCons (method_decl.pre mdecl') ?\<omega>0_rets_empty"
+            unfolding assertion_framing_state_def \<comment>\<open>using that the precondition is self-framing\<close>
+          proof (rule allI | rule impI)+
+            fix res
+            assume "red_inhale ctxt_vpr StateCons (method_decl.pre mdecl') ?\<omega>0_rets_empty res"
+            with StoreWellTy HeapWellTy EmptyState
+            show "res \<noteq> RFailure"
+              using MethodSpecsFramed
+              unfolding vpr_method_spec_correct_total_def vpr_method_correct_total_aux_def \<open>mdecl = _\<close>
+              by blast
+          qed
+          moreover have ValidRes: "StateCons (?\<omega>0_rets \<ominus> ?\<omega>pre_exh_aux_rets) \<and> valid_heap_mask (get_mh_total_full (?\<omega>0_rets \<ominus> ?\<omega>pre_exh_aux_rets))"
+          proof (rule conjI)
+            let ?\<omega>minus = "?\<omega>0_rets \<ominus> ?\<omega>pre_exh_aux_rets"
+            have gt_\<omega>minus: "?\<omega>0_rets \<succeq> ?\<omega>minus"
+            using \<open>?\<omega>0_rets \<succeq> ?\<omega>pre_exh_aux_rets\<close> minus_smaller 
+            by auto
+
+            show "StateCons ?\<omega>minus"
+            proof (rule mono_prop_downwardD[OF wf_total_consistency_trace_mono_downwardD[OF WfConsistency] _ gt_\<omega>minus])
+              show "StateCons ?\<omega>0_rets"
+                apply (rule total_consistency_store_update[OF WfConsistency])
+                using state_rel_consistent StateRelDuringCall ConsistencyEnabled
+                apply fastforce
+                by simp_all
+            qed
+          
+            show "valid_heap_mask (get_mh_total_full ?\<omega>minus)"
+              apply (rule valid_heap_mask_downward_mono)
+               apply (rule state_rel_wf_mask_simple[OF StateRelDuringCall])
+              using gt_\<omega>minus full_total_state_greater_mask 
+              by fastforce
+          qed
+          moreover have "mono_prop_downward StateCons"
+            using ConsistencyDownwardMono mono_prop_downward_ord_implies_mono_prop_downward 
+            by auto
+          ultimately show ?thesis
+            using exhale_inhale_normal MethodSpecSubset \<open>mdecl = _\<close>
+            by blast
+        qed
+        ultimately have PostFramedAuxSmaller: "vpr_postcondition_framed ctxt_vpr StateCons (method_decl.post mdecl) (get_total_full (?\<omega>0_rets \<ominus> ?\<omega>pre_exh_aux_rets)) (get_store_total ?\<omega>0_rets)"
+          using MethodSpecsFramed
+          unfolding vpr_method_spec_correct_total_def vpr_method_correct_total_aux_def
+          by fastforce
+
+        have PostFramedAux: "vpr_postcondition_framed ctxt_vpr StateCons (method_decl.post mdecl) (get_total_full \<omega>) (get_store_total ?\<omega>0_rets)"
+        proof -
+          have "(get_total_full (?\<omega>0_rets \<ominus> ?\<omega>pre_exh_aux_rets)) \<le> (get_total_full \<omega>)"
+            by (metis \<open>?\<omega>0_rets \<succeq> ?\<omega>pre_exh_aux_rets\<close> full_total_state.select_convs(3) full_total_state.update_convs(1) greater_full_total_state_total_state minus_smaller total_state_greater_equiv)
+          thus ?thesis
+            using vpr_postcondition_framed_mono ConsistencyDownwardMono MethodSpecSubset PostFramedAuxSmaller 
+            by blast
+        qed
+
+      show ?thesis
+      unfolding assertion_framing_state_def
+      proof (rule allI, rule impI)+
+        let ?\<phi>havoc = "get_total_full ?\<omega>havoc"
+        let ?\<omega>havoc2 = "\<lparr> get_store_total = get_store_total ?\<omega>0_rets, 
+                          get_trace_total = [old_label \<mapsto> get_total_full \<omega>],
+                          get_total_full = ?\<phi>havoc \<rparr>"
+
+          fix res
+          assume "red_inhale ctxt_vpr StateCons (method_decl.post mdecl) ?\<omega>havoc res"
+          hence "red_inhale ctxt_vpr StateCons (method_decl.post mdecl) ?\<omega>havoc2 res"
+            by auto
+          moreover have "total_heap_well_typed (program_total ctxt_vpr) (absval_interp_total ctxt_vpr) (get_hh_total ?\<phi>havoc)"
+            using state_rel_heap_var_rel[OF \<open>?RCallPost ?\<omega>havoc ?nshavoc\<close>] \<open>Pr = _\<close> \<open>domain_type TyRep = _\<close>
+            unfolding heap_var_rel_def
+            by simp
+          moreover have "valid_heap_mask (get_mh_total ?\<phi>havoc)"
+            using \<open>?RCallPost ?\<omega>havoc ?nshavoc\<close> state_rel_wf_mask_simple
+            by fastforce
+          ultimately show "res \<noteq> RFailure"
+            using PostFramedAux
+            unfolding vpr_postcondition_framed_def
+            using assertion_framing_state_def 
+            by (metis fun_upd_same)                     
+        qed
+      qed
+
+      note RCallPostConj = conjI[OF \<open>?RCallPost ?\<omega>havoc ?nshavoc\<close> PostFramed]     
+
+      show ?thesis  
+      proof (cases resPost)
+        case RMagic
+        then show ?thesis \<comment>\<open>trivial case\<close>
+          using \<open>res = _\<close>
+          by (auto intro: rel_vpr_aux_intro)
+      next
+        case RFailure
+          with RedInh stmt_rel_failure_elim[OF InhalePostRelInst RCallPostConj] \<open>mdecl = _\<close>
+          obtain c where 
+              "red_ast_bpl P ctxt (?\<gamma>pre, Normal nspre) c" and
+              "snd c = Failure"
+            using RedBplHavoc red_ast_bpl_transitive
+            by blast
+          moreover from RFailure \<open>res = _\<close> have "res = RFailure"
+            by simp
+          ultimately show ?thesis 
+            using RedBplPre red_ast_bpl_transitive
+            by (blast intro: rel_vpr_aux_intro)
+      next
+        case (RNormal \<omega>post)
+          with RedInh stmt_rel_normal_elim[OF InhalePostRelInst RCallPostConj] \<open>mdecl = _\<close>
+          obtain nspost where 
+              "red_ast_bpl P ctxt (?\<gamma>pre, Normal nspre) (\<gamma>', Normal nspost)" and
+              "?RCallPost \<omega>post nspost"
+            using RedBplHavoc red_ast_bpl_transitive
+            by blast
+          hence "red_ast_bpl P ctxt (\<gamma>, Normal ns) (\<gamma>', Normal nspost)"
+            using RedBplPre red_ast_bpl_transitive
+            by blast
+
+          moreover have "get_store_total \<omega>post = get_store_total ?\<omega>havoc"
+          using RedMethodCall \<open>resPre = _\<close> \<open>resPost = _\<close> inhale_only_changes_mask(3)
+          by (metis RedInhale_case sub_expressions.simps(7))
+
+          moreover from RNormal \<open>res = _\<close> have "res = RNormal (reset_state_after_call ys v_rets \<omega> \<omega>post)"
+            by simp
+            
+          moreover have                                          
+             "state_rel_def_same Pr StateCons TyRep Tr AuxPred ctxt (reset_state_after_call ys v_rets \<omega> \<omega>post) nspost"
+          proof -
+            from \<open>?RCallPost \<omega>post nspost\<close> have
+              "state_rel_def_same Pr StateCons TyRep (Tr\<lparr>var_translation := var_tr''\<rparr>) AuxPred ctxt \<omega>post nspost"
+              apply (rule state_rel_aux_pred_remove)
+              apply (rule map_upd_set_subset2)
+              using var_translation_disjoint[OF StateRelConcrete[OF \<open>R \<omega> ns\<close>]]
+              by blast
+
+            thus ?thesis
+            proof (rule state_rel_store_update[where ?f="var_translation Tr"])
+              show "store_rel (type_interp ctxt) (var_context ctxt) (var_translation Tr) 
+                              (reset_state_after_call ys v_rets \<omega> \<omega>post) nspost"
+              proof (rule store_relI)
+                show "inj_on (var_translation Tr) (dom (var_translation Tr))"
+                  using state_rel_store_rel[OF StateRelConcrete[OF \<open>R \<omega> ns\<close>]]
+                  by (simp add: store_rel_def)
+              next
+                fix var_vpr var_bpl
+                assume VarTrSome: "var_translation Tr var_vpr = Some var_bpl"
+                show "store_var_rel_aux (type_interp ctxt) (var_context ctxt) (reset_state_after_call ys v_rets \<omega> \<omega>post) nspost var_vpr var_bpl"
+                proof (cases "var_vpr \<in> set ys")
+                  case True
+                  from this obtain id where "var_vpr = ys ! id" and "id < length ys"
+                    by (metis in_set_conv_nth)
+                  hence "var_bpl = ys_bpl ! id"
+                    using YsBplEq VarTrSome
+                    by auto
+
+                  have *: "(length es + id) = [0..<length es + length ys] ! (length es + id)"
+                    using \<open>id < _\<close> LengthEqs
+                    by auto
+
+                  have "var_tr'' (length es + id) = Some var_bpl"
+                    using \<open>id < _\<close> LengthEqs map_upds_distinct_nth[OF distinct_upt *, 
+                                                                   where ?m=Map.empty and ?ys="xs_bpl @ ys_bpl"]
+                    unfolding \<open>var_tr'' = _\<close> \<open>var_bpl = (ys_bpl ! id)\<close>
+                    by (smt (verit) True add.commute add_less_cancel_right diff_less diff_zero length_append length_pos_if_in_set length_rev length_upt nth_append_length_plus rev_append zero_less_Suc)
+
+                  from this obtain val_vpr ty_bpl where
+                    AuxStoreRel:
+                     "get_store_total \<omega>post (length es + id) = Some val_vpr \<and>
+                     lookup_var (var_context ctxt) nspost var_bpl = Some (val_rel_vpr_bpl val_vpr) \<and>
+                     lookup_var_ty (var_context ctxt) var_bpl = Some ty_bpl \<and>
+                     type_of_val (type_interp ctxt) (val_rel_vpr_bpl val_vpr) = ty_bpl"
+                    using state_rel_store_rel[OF \<open>?RCallPost \<omega>post nspost\<close>]
+                    unfolding store_rel_def
+                    by auto
+
+                  have "val_vpr = v_rets ! id"
+                  proof -
+                    have *: "(length es + id) < length (v_args @ v_rets)"
+                              using \<open>id < _\<close> LengthEqs
+                              by simp
+                    have "get_store_total \<omega>post (length es + id) = shift_and_add_list_alt Map.empty (v_args @ v_rets) (length es + id)"
+                        by (simp add: \<open>get_store_total \<omega>post = _\<close>)
+                    also have "... = Some ((v_args @ v_rets) ! (length es + id))"
+                      using \<open>id < _\<close> shift_and_add_list_alt_lookup_1[OF *] 
+                      by blast
+                    also have "... = Some (v_rets ! id)"
+                      using LengthEqs
+                      by fastforce
+                    finally show ?thesis
+                      using AuxStoreRel
+                      by auto  
+                  qed
+                     
+                  show ?thesis
+                  unfolding store_var_rel_aux_def
+                  proof ((rule exI)+, intro conjI)
+                    show "get_store_total (reset_state_after_call ys v_rets \<omega> \<omega>post) var_vpr = Some (v_rets ! id)"
+                      unfolding reset_state_after_call_def
+                      apply simp
+                      using \<open>var_vpr = _\<close> \<open>distinct ys\<close> map_upds_distinct_nth \<open>id < _\<close> LengthEqs
+                      by metis
+                  next
+                    show "lookup_var (var_context ctxt) nspost var_bpl = Some (val_rel_vpr_bpl (v_rets ! id))"
+                      using AuxStoreRel \<open>val_vpr = v_rets ! id\<close>                                           
+                      by simp
+                  next
+                    show "lookup_var_ty (var_context ctxt) var_bpl = Some ty_bpl"
+                      using AuxStoreRel
+                      by blast
+                  next
+                    show "type_of_val (type_interp ctxt) (val_rel_vpr_bpl (v_rets ! id)) = ty_bpl"
+                      using AuxStoreRel\<open>val_vpr = v_rets ! id\<close>
+                      by blast
+                  qed
+                next
+                  case False
+                  \<comment>\<open>In this case, \<^term>\<open>var_vpr\<close> is not a target variable and thus we need to show that
+                     it still contains the same value as before the call. \<close>
+
+                  hence "var_bpl \<notin> set ys_bpl"
+                    using map_the_inj_not_in state_rel_var_tr_inj[OF StateRelConcrete[OF \<open>R \<omega> ns\<close>]]
+                          YsBplEq VarTrSome \<open>set ys \<subseteq> _\<close>
+                    by fast
+
+                  have "get_store_total (reset_state_after_call ys v_rets \<omega> \<omega>post) var_vpr = 
+                         get_store_total \<omega> var_vpr"
+                    unfolding reset_state_after_call_def
+                    by (simp add: False)
+
+                  moreover have "lookup_var (var_context ctxt) nspost var_bpl = 
+                                 lookup_var (var_context ctxt) ns var_bpl"
+                  proof -
+                    from VarTrSome obtain v_bpl where 
+                      LookupVarBpl: "lookup_var (var_context ctxt) ns var_bpl = Some v_bpl"
+                      using state_rel_store_rel[OF StateRelConcrete[OF \<open>R \<omega> ns\<close>]]
+                      unfolding store_rel_def
+                      by blast                    
+
+                    show ?thesis
+                    proof (cases "var_vpr \<in> set xs")
+                      case True
+                      \<comment>\<open>In this case, \<^term>\<open>var_vpr\<close> is an argument variable, which means the proof
+                         tracked the corresponding Boogie variable in the variable translation. Thus,
+                         by showing that the Viper local store did not change during the call (except
+                         for target variables), we can show that the Boogie variable was not modified either.\<close>
+
+                      have "var_bpl \<in> set xs_bpl"
+                      proof -
+                        from \<open>var_vpr \<in> set xs\<close> obtain i where
+                             "i < length xs" and "xs ! i = var_vpr"
+                          by (meson in_set_conv_nth)
+
+                        thus ?thesis
+                          using XsBplEq VarTrSome LengthEqs
+                          by (metis comp_eq_dest_lhs nth_map nth_mem option.sel)
+                      qed
+
+                      from this obtain i where "i < length xs_bpl" and "var_bpl = xs_bpl ! i"
+                        by (metis in_set_conv_nth)
+
+                      hence *: "i = [0..<length es+length ys] ! i"
+                        using LengthEqs
+                        by fastforce
+
+                      have "var_tr'' i = Some var_bpl"
+                        using map_upds_distinct_nth[OF distinct_upt *, where ?m=Map.empty and ?ys="xs_bpl@ys_bpl"] 
+                              LengthEqs
+                        unfolding \<open>var_tr'' = _\<close> \<open>var_bpl = _\<close>
+                        using \<open>i < _\<close>
+                        by (simp add: nth_append)
+                                                                                              
+                      with state_rel_store_rel[OF \<open>?RCallPost \<omega>post nspost\<close>] obtain val_vpr where 
+                        "get_store_total \<omega>post i = Some val_vpr" and
+                        "lookup_var (var_context ctxt) nspost var_bpl = Some (val_rel_vpr_bpl val_vpr)"
+                        unfolding store_rel_def
+                        by auto
+
+                      hence "lookup_var (var_context ctxt) nspost var_bpl = Some (val_rel_vpr_bpl (v_args ! i))"
+                        unfolding \<open>get_store_total \<omega>post = _\<close>
+                        using \<open>i < _\<close> LengthEqs
+                        by (simp add: shift_and_add_list_alt_lookup nth_append)
+
+                      moreover from ValRelArgs have
+                        "lookup_var (var_context ctxt) ns var_bpl = Some (val_rel_vpr_bpl (v_args ! i))"
+                        using \<open>var_bpl = _\<close>
+                        by (simp add: \<open>i < length xs_bpl\<close> list_all2_conv_all_nth)
+
+                      ultimately show ?thesis
+                        by simp
+                    next
+                      case False
+                      \<comment>\<open>In this case, \<^term>\<open>var_vpr\<close> is not an argument variable or target variable.
+                         Thus, the proof tracked the corresponding Boogie variable explicitly as an 
+                         auxiliary variable that must still have the same value as before the call.\<close>
+                      
+                      hence "var_bpl \<notin> set xs_bpl" 
+                        using map_the_inj_not_in state_rel_var_tr_inj[OF StateRelConcrete[OF \<open>R \<omega> ns\<close>]]
+                              XsBplEq VarTrSome \<open>set xs \<subseteq> _\<close>
+                        by fast
+                                             
+                      have *: "map_upd_set AuxPred (ran (var_translation Tr) - (set xs_bpl \<union> set ys_bpl))
+                               ?fpred var_bpl = Some (?fpred var_bpl)"
+                        apply (rule map_upd_set_lookup_1)
+                        using \<open>var_bpl \<notin> set xs_bpl\<close> \<open>var_bpl \<notin> set ys_bpl\<close> VarTrSome
+                              ranI
+                        by fast
+
+                      thus ?thesis
+                        using state_rel_aux_pred_sat_lookup[OF \<open>?RCallPost \<omega>post nspost\<close> *]
+                              LookupVarBpl
+                        unfolding pred_eq_def
+                        by (simp add: has_Some_iff)
+                      qed                   
+                    qed
+                  ultimately show ?thesis
+                    using VarTrSome state_rel_store_rel[OF StateRelConcrete[OF \<open>R \<omega> ns\<close>]]
+                    unfolding store_var_rel_aux_def store_rel_def
+                    by presburger                    
+                qed
+              qed
+            next
+              have "StateCons_t (get_total_full \<omega>post)"
+              proof -
+                have "consistent_state_rel_opt (state_rel_opt (Tr\<lparr>var_translation := var_tr''\<rparr>))"
+                  by (simp add: ConsistencyEnabled)
+
+                with \<open>?RCallPost \<omega>post _\<close> state_rel_consistent WfConsistency 
+                show ?thesis
+                unfolding wf_total_consistency_def                
+                by blast
+              qed
+
+              show "StateCons (reset_state_after_call ys v_rets \<omega> \<omega>post)"
+                unfolding reset_state_after_call_def
+                apply (rule total_consistencyI[OF WfConsistency])
+                 apply (simp add: \<open>StateCons_t (get_total_full \<omega>post)\<close>)                 
+                using state_rel_consistent[OF StateRel] WfConsistency ConsistencyEnabled
+                unfolding wf_total_consistency_def
+                by simp
+            next
+              show "binder_state nspost = Map.empty"
+                using state_rel_state_well_typed[OF \<open>?RCallPost \<omega>post nspost\<close>, simplified state_well_typed_def]
+                by simp
+            next
+              show "ran (var_translation Tr) \<inter>
+                   ({heap_var (Tr\<lparr>var_translation := var_tr''\<rparr>), heap_var_def (Tr\<lparr>var_translation := var_tr''\<rparr>)} \<union>
+                    {mask_var (Tr\<lparr>var_translation := var_tr''\<rparr>), mask_var_def (Tr\<lparr>var_translation := var_tr''\<rparr>)} \<union>
+                    ran (field_translation (Tr\<lparr>var_translation := var_tr''\<rparr>)) \<union>
+                    range (const_repr (Tr\<lparr>var_translation := var_tr''\<rparr>)) \<union>
+                    dom AuxPred) =
+                   {}"
+                using var_translation_disjoint[OF StateRelConcrete[OF \<open>R \<omega> ns\<close>]]
+                by simp
+            qed (simp_all add: reset_state_after_call_def)
+              
+          qed
+            
+          ultimately show ?thesis 
+            by (blast intro: rel_vpr_aux_intro)
+        qed
+      qed
+  next
+    case RedSubExpressionFailure
+    \<comment>\<open>Since the arguments are assumed to be arguments, this case cannot occur\<close>
+    have SubExpEq: "sub_expressions (MethodCall ys m es) = map ViperLang.Var xs"
+      by (simp add: \<open>es = _\<close>) 
+
+    from RedSubExpressionFailure
+    show ?thesis
+      unfolding SubExpEq
+    proof -
+      assume "red_pure_exps_total ctxt_vpr StateCons (Some \<omega>) (map pure_exp.Var xs) \<omega> None"
+
+      from this obtain i where 
+        "ctxt_vpr, StateCons, Some \<omega> \<turnstile> \<langle>pure_exp.Var (xs ! i); \<omega>\<rangle> [\<Down>]\<^sub>t VFailure"
+        using red_exp_list_failure_nth
+        by (metis SubExpEq length_map local.RedSubExpressionFailure(2) nth_map)
+        
+      hence False
+        by (cases) auto
+
+      thus ?thesis
+        by simp
+    qed
+  qed
+qed
+
+
+end
